More restructuring of proofs

proof/X-Wing-Correction-Proof.ec
@@ -3,84 +3,130 @@ require import AllCore IntDiv CoreMap List Distr IntDiv StdOrder.
 from Jasmin require import JModel_x86 JWord JUtils.
 
 import SLH64 StdOrder.IntOrder.
-require import Jkem_avx2_clean XWing_Spec XWing_Helper_Functions CorrectnessProof_Mulx Mulx_scalarmult_s Jkem_avx2_stack FIPS202_SHA3 MLKEM Curve25519_Procedures.
-require import Array4 Array6 Array8 Array32 Array64 Array96 Array140 Array152 Array1088 Array1120 Array1184 Array1216 Array2400.
+require import Xkem_avx2_clean XWing_Spec XWing_Helper_Functions CorrectnessProof_Mulx Mulx_scalarmult_s Jkem_avx2_stack FIPS202_SHA3 Curve25519_Procedures MLKEM MLKEM_KEM_avx2_stack.
+require import Array4 Array6 Array8 Array32 Array64 Array96 Array140 Array152 Array1088 Array1120 Array1184 Array1216 Array2400 Array1152.
 require import WArray4 WArray6 WArray32 WArray64 WArray96 WArray1088 WArray1120 WArray1184 WArray1216 WArray2400.
 
-op SHA3_256_A128_A6 : W8.t Array32.t -> W8.t Array32.t -> W8.t Array32.t -> W8.t Array32.t -> W8.t Array32.t -> W8.t Array32.t.
-op SHAKE256_A96_A32 : W8.t Array96.t -> W8.t Array32.t -> W8.t Array96.t.
-
+axiom shake256_A96_A32 out inp :
+   phoare [Xkem_avx2_clean.M._shake256_A96__A32 :
+               arg = (out, inp) ==>
+               res = SHAKE256_32_96 inp] = 1%r.
 
 axiom sha3_256_A128__A6 ss ss_mlkem ss_x25519 ct_25519 pk_25519 :
-   phoare [Jkem_avx2_clean.M._sha3_256_A128__A6 :
+   phoare [Xkem_avx2_clean.M._sha3_256_A128__A6 :
                arg = (ss, ss_mlkem, ss_x25519, ct_25519, pk_25519) ==>
-               res = SHA3_256_A128_A6 ss ss_mlkem ss_x25519 ct_25519 pk_25519] = 1%r.
+               res = SHA3_256_134_32 (ss_mlkem, ss_x25519, ct_25519, pk_25519, xwing_label)] = 1%r.
 
-axiom shake256_A96_A32 out inp :
-   phoare [Jkem_avx2_clean.M._shake256_A96__A32 :
-               arg = (out, inp) ==>
-               res = SHAKE256_A96_A32 out inp] = 1%r.
 
-abbrev toRep4 (x: W8.t Array32.t) = Array4.init (fun (i : int) => get64 (WArray32.init8 (fun (i0 : int) => x.[i0])) i).
-abbrev toRep32 (x: W64.t Array4.t) = Array32.init (fun (i : int) => get8 (WArray32.init64 (fun (i0 : int) => x.[i0])) i).
+abbrev toRep4 (x: W8.t Array32.t) = Array4.of_list W64.zero (to_list (unpack64 (pack32 (to_list x)))).
 
 lemma xwing_25519_base_mulx_equiv :
-   equiv [Jkem_avx2_clean.M.xwing_x25519_base ~ Mulx_scalarmult_s.M.__curve25519_mulx_base :
+   equiv [Xkem_avx2_clean.M.xwing_x25519_base ~ Mulx_scalarmult_s.M.__curve25519_mulx_base :
        _k{2} = toRep4 np{1}
        ==>
-       res{1} = toRep32 res{2}].
+       res{2} = toRep4 res{1}].
     proc.
     inline{1} 4.
     seq 7 3 : (={u, r, k, _k}). wp. auto => />.
+    move => &1.
+    + rewrite unpack64E pack32E /init8 of_listE.
+    + rewrite tP => i ib.
+    + rewrite initiE 1:/# /= /get8 /(\bits64).
+    + rewrite initiE 1:/# /= /copy_64.
+    + rewrite initiE 1:/# /= /get64_direct.
+    + rewrite /pack8_t. rewrite wordP => ii iib.
+    + rewrite initiE 1:/# //= initiE 1:/# //=.
+    + rewrite initiE 1:/# //= initiE 1:/# //=.
+    + rewrite  initiE 1:/# //= initiE 1:/# //=.
+    + rewrite /to_list /mkseq -iotaredE => />.
+    + smt().
     seq 4 3 : (={u, k, _k, r} /\ q{1} = r{2}). sim.
     wp; skip => />.
+    move => &2.
+    + rewrite unpack64E pack32E of_listE.
+    + rewrite tP => i ib.
+    + rewrite initiE 1:/# /= /get8 /(\bits64).
+    + rewrite initiE 1:/# /= /copy_64.
+    + rewrite wordP => ii iib.
+    + rewrite initiE 1:/# /= /init64 /(\bits8).
+    + rewrite initiE 1:/# //= initiE 1:/# //=.
+    + rewrite /to_list /mkseq -iotaredE => />.
+    + smt(W8.initiE).
 qed.
 
 lemma xwing_25519_mulx_equiv :
-   equiv [Jkem_avx2_clean.M.xwing_x25519 ~ Mulx_scalarmult_s.M.__curve25519_mulx :
+   equiv [Xkem_avx2_clean.M.xwing_x25519 ~ Mulx_scalarmult_s.M.__curve25519_mulx :
        _k{2} = toRep4 np{1}  /\
        _u{2} = toRep4 pp{1}
        ==>
-       res{1} = toRep32 res{2}].
+       res{2} = toRep4 res{1}].
     proc.
     inline{1} 6.
     wp; sp.
     sim :  (={k, u, r}).
+    move => &1 &2 [?] [H] *. rewrite H.
+    + rewrite unpack64E pack32E /init8 of_listE.
+    + rewrite tP => i ib.
+    + rewrite initiE 1:/# /= /get8 /(\bits64).
+    + rewrite initiE 1:/# /= /copy_64.
+    + rewrite /to_list /init64 /(\bits8) /get64_direct /mkseq -iotaredE => />.
+    + rewrite wordP => ii iib.
+    + rewrite initiE 1:/# /=.
+    + rewrite initiE 1:/# //= initiE 1:/# //=.
+    ring. smt(W8.initiE).
+    auto => />. move => &1 *.
+    do split.
+    + rewrite unpack64E pack32E of_listE.
+    + rewrite tP => i ib.
+    + rewrite initiE 1:/# /= /get8 /(\bits64).
+    + rewrite initiE 1:/# /= /copy_64 /get64_direct.
+    + rewrite wordP => ii iib.
+    + rewrite initiE 1:/# /= /init64 /(\bits8) /pack8_t.
+    + rewrite !initiE 1,2:/# //=  initiE 1:/# //= initiE 1:/# //=.
+    + rewrite initiE 1:/# //= initiE 1:/# //=.
+    + rewrite /to_list /mkseq -iotaredE => />. smt().
+    + rewrite unpack64E pack32E of_listE.
+    + rewrite tP => i ib.
+    + rewrite initiE 1:/# /= /get8 /(\bits64).
+    + rewrite initiE 1:/# /= /copy_64 /get64_direct.
+    + rewrite wordP => ii iib.
+    + rewrite initiE 1:/# /= /init64 /(\bits8) /pack8_t.
+    + rewrite !initiE 1,2:/# //=  initiE 1:/# //= initiE 1:/# //=.
+    + rewrite initiE 1:/# //= initiE 1:/# //=.
+    + rewrite /to_list /mkseq -iotaredE => />. smt().
 qed.
 
 lemma eq_spec_xwing_25519_base_mulx :
-   equiv [Jkem_avx2_clean.M.xwing_x25519_base ~ CurveProcedures.scalarmult_base :
+   equiv [Xkem_avx2_clean.M.xwing_x25519_base ~ CurveProcedures.scalarmult_base :
        Array4.of_list W64.zero (to_list (unpack64 k'{2})) = toRep4 np{1}
        ==>
-       pack32 (to_list res{1}) = res{2}
+       Array32.of_list W8.zero (to_list (unpack8 res{2})) = res{1}
    ].
     transitivity
     Mulx_scalarmult_s.M.__curve25519_mulx_base
-    (toRep4 np{1} = _k{2} ==> res{1} = toRep32 res{2})
+    (toRep4 np{1} = _k{2} ==> toRep4 res{1} =  res{2})
     (pack4 (to_list _k{1}) = k'{2} ==> pack4 (to_list res{1}) = res{2}) => />.
     move => &1 &2 H.
     exists(Array4.of_list W64.zero (to_list (unpack64 k'{2}))).
     do split.
     + by rewrite -H. by rewrite of_listK.
     move => &m.
-    rewrite of_listE /of_list pack32E pack4E /get8 /init64 !/to_list /(\bits8) /mkseq -iotaredE => />.
-    congr. apply fun_ext => i. rewrite !initE => />.
-    + case( 0 <= i %/ 8 && i %/ 8 < 32) => C. smt(W8.initiE). by rewrite ifF 1:/#.
-   proc *. by call xwing_25519_base_mulx_equiv.
-   proc *. symmetry. by call eq_spec_impl_scalarmult_base_mulx.
+    rewrite of_listK //=  of_listK //=. rewrite size_to_list //=. rewrite to_listK //=.
+    proc *. by call xwing_25519_base_mulx_equiv.
+    proc *. symmetry. by call eq_spec_impl_scalarmult_base_mulx.
 qed.
 
 lemma eq_spec_xwing_25519_mulx :
-   equiv [Jkem_avx2_clean.M.xwing_x25519 ~ CurveProcedures.scalarmult :
+   equiv [Xkem_avx2_clean.M.xwing_x25519 ~ CurveProcedures.scalarmult :
        Array4.of_list W64.zero (to_list (unpack64 k'{2})) = toRep4 np{1} /\
        Array4.of_list W64.zero (to_list (unpack64 u'{2})) = toRep4 pp{1}
        ==>
-       pack32 (to_list res{1}) = res{2}
+       Array32.of_list W8.zero (to_list (unpack8 res{2})) = res{1}
    ].
     transitivity
     Mulx_scalarmult_s.M.__curve25519_mulx
     (toRep4 np{1} = _k{2} /\ toRep4 pp{1} = _u{2}
-     ==> res{1} = toRep32 res{2})
+     ==> toRep4 res{1} = res{2})
     (pack4 (to_list _k{1}) = k'{2} /\
      pack4 (to_list _u{1}) = u'{2}
      ==> pack4 (to_list res{1}) = res{2}) => />.
@@ -89,10 +135,29 @@ lemma eq_spec_xwing_25519_mulx :
     do split.
     + by rewrite -H. by rewrite -H0. by rewrite //= of_listK. by rewrite //= of_listK.
     move => &m.
-    rewrite of_listE /of_list pack32E pack4E /get8 /init64 /to_list /(\bits8) /mkseq -iotaredE => />.
-    congr. apply fun_ext => i. rewrite !initE => />.
-    + case( 0 <= i %/ 8 && i %/ 8 < 32) => C. smt(W8.initiE). by rewrite ifF 1:/#.
+    rewrite of_listK //=  of_listK //=. rewrite size_to_list //=. rewrite to_listK //=.
+    proc *. by call xwing_25519_mulx_equiv.
+    proc *. symmetry. by call eq_spec_impl_scalarmult_mulx.
+qed.
 
-   proc *. by call xwing_25519_mulx_equiv.
-   proc *. symmetry. by call eq_spec_impl_scalarmult_mulx.
+lemma eq_spec_xwing_keygen:
+  equiv [Xkem_avx2_clean.M.jade_kem_xwing_xwing_amd64_avx2_keypair_derand ~ XWing.kg_derand :
+      sk{2} = coins{1}
+      ==>
+      res{1}.`2 = res{2}.`1 /\
+      res{1}.`1 = Array1216.of_list W8.zero (to_list (res{2}.`2).`1.`1 ++ to_list (res{2}.`2).`1.`2 ++ to_list (res{2}.`2).`2)
+
+  ].
+  proc. inline {2} 1. inline {1} 2. wp.
+  do 3! unroll for{1} ^while. wp.
+  swap{1} 15 2.
+  call eq_spec_xwing_25519_base_mulx; wp.
+  call mlkem_kem_correct_internal_kg; wp.
+  ecall{1} (shake256_A96_A32 expanded{1} srandomness{1}); wp.
+  skip; auto => />. move => &1.
+  do split.
+  admit. (* this needs to change in the jasmin extraction, provable but takes forever. *)
+  admit. (* this needs to change in the jasmin extraction, provable but takes forever. *)
+  move => *.
+  admit. (* this needs to change in the jasmin extraction, too big to be provable imo. *)
 qed.
